Dafny/Request.dfy
@@ -1,8 +1,12 @@
-include "Blood.dfy"
-
-datatype request = request(type: string, volume: int)
+include "BloodInventory.dfy"
+include "Alert.dfy"
+datatype request = bloodRequest(bloodType: string, volume: int)
 
 method Request(batchRequest:array<request>, bloodInventory: BloodInventory)
+requires batchRequest != null
+requires bloodInventory != null
+requires forall i :: 0 <= i < batchRequest.Length ==> (validBloodType(batchRequest[i].bloodType))
+requires forall i :: 0 <= i < batchRequest.Length ==> (batchRequest[i].volume >= bloodInventory.GetBloodCountForBloodTypeVerification(batchRequest[i].bloodType, bloodInventory.GetSizeVerificaiton()))
 {
-    
+
 }
